ott_coq/destination_calculus_proofs.v
@@ -5,15 +5,51 @@ Require Import Ott.destination_calculus_notations.
 Require Import Ott.ext_nat.
 Require Import Coq.Program.Equality.
 
-Lemma UnionPreservesNames : forall (G1 G2: ctx), (forall (n : name), CtxM.In n G1 -> CtxM.In n (G1 ⨄ G2)) /\ (forall (n : name), CtxM.In n G1 -> CtxM.In n (G1 ⨄ G2)).
+Lemma UnionPreservesNames : forall (G1 G2: ctx), (forall (n : name), CtxM.In n G1 -> CtxM.In n (G1 ⨄ G2)) /\ (forall (n : name), CtxM.In n G2 -> CtxM.In n (G1 ⨄ G2)). Proof. Admitted.
+Lemma UnionPropagatesNames : forall (G1 G2: ctx), (forall (n : name), CtxM.In n (G1 ⨄ G2) -> CtxM.In n G1 \/ CtxM.In n G2). Proof. Admitted.
+Lemma UnionPreservesNoVar : forall (G1 G2: ctx), ctx_NoVar G1 -> ctx_NoVar G2 -> ctx_NoVar (G1 ⨄ G2). Proof. Admitted.
+Lemma UnionPropagatesNoVar : forall (G1 G2: ctx), ctx_NoVar (G1 ⨄ G2) -> ctx_NoVar G1 * ctx_NoVar G2. Proof. Admitted.
+Lemma UnionPreservesNoHole : forall (G1 G2: ctx), ctx_NoHole G1 -> ctx_NoHole G2 -> ctx_NoHole (G1 ⨄ G2). Proof. Admitted.
+Lemma UnionPropagatesNoHole : forall (G1 G2: ctx), ctx_NoHole (G1 ⨄ G2) -> ctx_NoHole G1 * ctx_NoHole G2. Proof. Admitted.
+Lemma UnionPreservesNoDest : forall (G1 G2: ctx), ctx_NoDest G1 -> ctx_NoDest G2 -> ctx_NoDest (G1 ⨄ G2). Proof. Admitted.
+Lemma UnionPropagatesNoDest : forall (G1 G2: ctx), ctx_NoDest (G1 ⨄ G2) -> ctx_NoDest G1 * ctx_NoDest G2. Proof. Admitted.
+Lemma UnionPropagatesValidity : forall (G1 G2: ctx), ctx_IsValid (G1 ⨄ G2) -> ctx_IsValid G1 * ctx_IsValid G2. Proof. Admitted.
+Lemma UnionPreservesDestOnly : forall (G1 G2: ctx), ctx_DestOnly G1 -> ctx_DestOnly G2 -> ctx_DestOnly (G1 ⨄ G2). Proof. Admitted.
+Lemma UnionPropagatesDestOnly : forall (G1 G2: ctx), ctx_DestOnly (G1 ⨄ G2) -> ctx_DestOnly G1 * ctx_DestOnly G2. Proof. Admitted.
+Lemma UnionPreservesVarOnly : forall (G1 G2: ctx), ctx_VarOnly G1 -> ctx_VarOnly G2 -> ctx_VarOnly (G1 ⨄ G2). Proof. Admitted.
+Lemma UnionPropagatesVarOnly : forall (G1 G2: ctx), ctx_VarOnly (G1 ⨄ G2) -> ctx_VarOnly G1 * ctx_VarOnly G2. Proof. Admitted.
+Lemma UnionPreservesHoleOnly : forall (G1 G2: ctx), ctx_HoleOnly G1 -> ctx_HoleOnly G2 -> ctx_HoleOnly (G1 ⨄ G2). Proof. Admitted.
+Lemma UnionPropagatesHoleOnly : forall (G1 G2: ctx), ctx_HoleOnly (G1 ⨄ G2) -> ctx_HoleOnly G1 * ctx_HoleOnly G2. Proof. Admitted.
+
+Lemma InteractPreservesNames : forall (G1 G2: ctx),
+    (
+        forall (n : name) (b:bndr),
+        CtxM.MapsTo n b G1 ->
+            CtxM.In n (G1 ⁻⨄⁺ G2) +
+            (sigT2 (fun b' => CtxM.MapsTo n b' G2) (fun b' => (bndr_Interact b b')))
+    ) * (
+        forall (n : name) (b':bndr),
+        CtxM.MapsTo n b' G2 ->
+            CtxM.In n (G1 ⁻⨄⁺ G2) +
+            (sigT2 (fun b => CtxM.MapsTo n b G1) (fun b => (bndr_Interact b b')))
+    ).
 Proof. Admitted.
-Lemma UnionPreservesNoHole : forall (G1 G2: ctx), ctx_NoHole G1 -> ctx_NoHole G2 -> ctx_NoHole (G1 ⨄ G2).
-Proof. Admitted.
-Lemma UnionPropagatesInvalidity : forall (G1 G2: ctx), ctx_Valid (G1 ⨄ G2) -> ctx_Valid G1 /\ ctx_Valid G2.
-Proof. Admitted.
-Lemma UnionPropagatesNoHole : forall (G1 G2: ctx), ctx_NoHole (G1 ⨄ G2) -> ctx_NoHole G1 /\ ctx_NoHole G2.
-Proof. Admitted.
-Lemma UnionDOVSingVarIsValid : forall (G : ctx) (x : tmv) (m : mode) (T : type), ctx_Valid G -> ctx_DestOnly G -> mode_Valid m -> ctx_Valid (G ⨄ ᶜ{ᵛ x ː m ‗ T}).
+Lemma InteractPropagatesNames : forall (G1 G2: ctx), (forall (n : name), CtxM.In n (G1 ⁻⨄⁺ G2) -> CtxM.In n G1 \/ CtxM.In n G2). Proof. Admitted.
+Lemma InteractPreservesNoVar : forall (G1 G2: ctx), ctx_NoVar G1 -> ctx_NoVar G2 -> ctx_NoVar (G1 ⁻⨄⁺ G2). Proof. Admitted.
+Lemma InteractPropagatesNoVar : forall (G1 G2: ctx), ctx_NoVar (G1 ⁻⨄⁺ G2) -> ctx_NoVar G1 * ctx_NoVar G2. Proof. Admitted.
+Lemma InteractPreservesNoHole : forall (G1 G2: ctx), ctx_NoHole G1 -> ctx_NoHole G2 -> ctx_NoHole (G1 ⁻⨄⁺ G2). Proof. Admitted.
+(* Lemma InteractPropagatesNoHole : forall (G1 G2: ctx), ctx_NoHole (G1 ⁻⨄⁺ G2) -> ctx_NoHole G1 * ctx_NoHole G2. Proof. Admitted. *)
+Lemma InteractPreservesNoDest : forall (G1 G2: ctx), ctx_NoDest G1 -> ctx_NoDest G2 -> ctx_NoDest (G1 ⁻⨄⁺ G2). Proof. Admitted.
+(* Lemma InteractPropagatesNoDest : forall (G1 G2: ctx), ctx_NoDest (G1 ⁻⨄⁺ G2) -> ctx_NoDest G1 * ctx_NoDest G2. Proof. Admitted. *)
+Lemma InteractPropagatesValidity : forall (G1 G2: ctx), ctx_IsValid (G1 ⁻⨄⁺ G2) -> ctx_IsValid G1 * ctx_IsValid G2. Proof. Admitted.
+Lemma InteractPreservesDestOnly : forall (G1 G2: ctx), ctx_DestOnly G1 -> ctx_DestOnly G2 -> ctx_DestOnly (G1 ⁻⨄⁺ G2). Proof. Admitted.
+(* Lemma InteractPropagatesDestOnly : forall (G1 G2: ctx), ctx_DestOnly (G1 ⁻⨄⁺ G2) -> ctx_DestOnly G1 * ctx_DestOnly G2. Proof. Admitted. *)
+Lemma InteractPreservesVarOnly : forall (G1 G2: ctx), ctx_VarOnly G1 -> ctx_VarOnly G2 -> ctx_VarOnly (G1 ⁻⨄⁺ G2). Proof. Admitted.
+Lemma InteractPropagatesVarOnly : forall (G1 G2: ctx), ctx_VarOnly (G1 ⁻⨄⁺ G2) -> ctx_VarOnly G1 * ctx_VarOnly G2. Proof. Admitted.
+Lemma InteractPreservesHoleOnly : forall (G1 G2: ctx), ctx_HoleOnly G1 -> ctx_HoleOnly G2 -> ctx_HoleOnly (G1 ⁻⨄⁺ G2). Proof. Admitted.
+(* Lemma InteractPropagatesHoleOnly : forall (G1 G2: ctx), ctx_HoleOnly (G1 ⁻⨄⁺ G2) -> ctx_HoleOnly G1 * ctx_HoleOnly G2. Proof. Admitted. *)
+
+Lemma UnionDOVSingVarIsValid : forall (G : ctx) (x : tmv) (m : mode) (T : type), ctx_IsValid G -> ctx_DestOnly G -> mode_IsValid m -> ctx_IsValid (G ⨄ ᶜ{ᵛ x ː m ‗ T}).
 Proof. Admitted.
 
 Lemma InteractPropagatesDestOnlyRight : forall (G1 G2: ctx), ctx_DestOnly (G1 ⁻⨄⁺ G2) -> ctx_DestOnly G2.
@@ -21,12 +57,12 @@ Proof. Admitted.
 
 Lemma StimesPropagatesNoHole : forall (m : mode) (G : ctx), ctx_NoHole (m ᶜ· G) -> ctx_NoHole G.
 Proof. Admitted.
-Lemma StimesPreservesValidity : forall (m : mode) (G : ctx), mode_Valid m -> ctx_Valid G -> ctx_Valid (m ᶜ· G).
+Lemma StimesPreservesValidity : forall (m : mode) (G : ctx), mode_IsValid m -> ctx_IsValid G -> ctx_IsValid (m ᶜ· G).
 Proof. Admitted.
-Lemma StimesPropagatesInvalidity : forall (m : mode) (G : ctx), ctx_Valid (m ᶜ· G) -> mode_Valid m /\ ctx_Valid G.
+Lemma StimesPropagatesInvalidity : forall (m : mode) (G : ctx), ctx_IsValid (m ᶜ· G) -> mode_IsValid m * ctx_IsValid G.
 Proof. Admitted.
 
-Lemma SubLemma : forall (G1 G2 : ctx) (x : tmv) (m : mode) (T1 T2 : type) (t : term) (v : val), (G1 ⨄ ᶜ{ᵛ x ː m ‗ T2} ᵗ⊢ t ː T1) -> (G2 ᵗ⊢ term_Val v ː T2) -> mode_Valid m -> ctx_Valid (G1 ⨄ (m ᶜ· G2)) -> ((G1 ⨄ (m ᶜ· G2)) ᵗ⊢ t ᵗ[ x ≔ v ] ː T1).
+Lemma SubLemma : forall (G1 G2 : ctx) (x : tmv) (m : mode) (T1 T2 : type) (t : term) (v : val), (G1 ⨄ ᶜ{ᵛ x ː m ‗ T2} ᵗ⊢ t ː T1) -> (G2 ᵗ⊢ term_Val v ː T2) -> mode_IsValid m -> ctx_IsValid (G1 ⨄ (m ᶜ· G2)) -> ((G1 ⨄ (m ᶜ· G2)) ᵗ⊢ t ᵗ[ x ≔ v ] ː T1).
 Proof. Admitted.
 
 Lemma BndrInSingleton : forall (b : bndr), CtxM.MapsTo (bndr_name b) b (ᶜ{b}).
@@ -53,15 +89,15 @@ Proof.
     - (* TyR_term_F *) admit.
     - (* TyR_term_Var *) admit.
     - (* TyR_term_App *)
-        intros d. rename H into Validm.
-        (* Get ctx_Valid G1, ctx_Valid G2 from ctx_Valid (m ᶜ· G1 ⨄ G2) *)
-        assert (ctx_Valid (m ᶜ· G1) /\ ctx_Valid G2) as ValidSG1G2. exact (UnionPropagatesInvalidity (m ᶜ· G1) G2 ValidG).
+        intros d. rename X into Validm.
+        (* Get ctx_IsValid G1, ctx_IsValid G2 from ctx_IsValid (m ᶜ· G1 ⨄ G2) *)
+        assert (ctx_IsValid (m ᶜ· G1) * ctx_IsValid G2) as ValidSG1G2. exact (UnionPropagatesValidity (m ᶜ· G1) G2 ValidG).
         destruct ValidSG1G2 as [ValidSG1 ValidG2].
         destruct (StimesPropagatesInvalidity m G1) as [Validm' ValidG1].
         exact ValidSG1.
         clear Validm'.
-        (* Get ctx_NoHole G1, ctx_noHole G2 from ctx_Valid (m ᶜ· G1 ⨄ G2) *)
-        assert (ctx_NoHole (m ᶜ· G1) /\ ctx_NoHole G2) as NoHoleSG1G2. exact (UnionPropagatesNoHole (m ᶜ· G1) G2 NoHoleG).
+        (* Get ctx_NoHole G1, ctx_noHole G2 from ctx_IsValid (m ᶜ· G1 ⨄ G2) *)
+        assert (ctx_NoHole (m ᶜ· G1) * ctx_NoHole G2) as NoHoleSG1G2. exact (UnionPropagatesNoHole (m ᶜ· G1) G2 NoHoleG).
         destruct NoHoleSG1G2 as [NoHoleSG1 NoHoleG2].
         assert (ctx_NoHole G1) as NoHoleG1. exact (StimesPropagatesNoHole m G1 NoHoleSG1).
         (* Get induction hypothesis and introduce v1 ⋄ e1 for t *)
@@ -76,10 +112,10 @@ Proof.
         destruct TSu'' as [REDu TYcmd2].
         destruct TYcmd1 as [Ge1 Gv1 v1 e1 T1 TYe1 TYv1 DestOnlyGe1v1].
         destruct TYe1 as [Ge1 e1 TYRe1 ValidGe1].
-        dependent destruction TYv1. rename G into Gv1, T into T1, TYRt into TYRv1, H into ValidGv1, H0 into NoHoleGv1.
-        dependent destruction TYcmd2. rename G1 into Ge2, G2 into Gv2, v into v2, e into e2, TYe into TYe2, TYv into TYv2, H into DestOnlyGe2v2.
+        dependent destruction TYv1. rename G into Gv1, T into T1, TYRt into TYRv1, X into ValidGv1, X0 into NoHoleGv1.
+        dependent destruction TYcmd2. rename G1 into Ge2, G2 into Gv2, v into v2, e into e2, TYe into TYe2, TYv into TYv2, X into DestOnlyGe2v2.
         destruct TYe2 as [Ge2 e2 TYRe2 ValidGe2].
-        dependent destruction TYv2. rename G into Gv2, TYRt into TYRv2, H into ValidGv2, H0 into NoHoleGv2.
+        dependent destruction TYv2. rename G into Gv2, TYRt into TYRv2, X into ValidGv2, X0 into NoHoleGv2.
         clear IHTYRt1. clear IHTYRt2. clear TSt. clear TSu.
         (* Canonical form on u *)
         inversion TYRv2.
@@ -91,16 +127,18 @@ Proof.
               unfold ctx_DestOnly in DestOnlyGv2.
               assert (CtxM.MapsTo (name_HD h) (⁻ h ː ¹ν ‗ T1 ⁔ m → T2) ᶜ{ ⁻ h ː ¹ν ‗ T1 ⁔ m → T2} -> bndr_IsDest (⁻ h ː ¹ν ‗ T1 ⁔ m → T2)). exact (DestOnlyGv2 (name_HD h) (⁻ h ː ¹ν ‗ T1 ⁔ m → T2)).
               assert (CtxM.MapsTo (name_HD h) (⁻ h ː ¹ν ‗ T1 ⁔ m → T2) ᶜ{ ⁻ h ː ¹ν ‗ T1 ⁔ m → T2}). exact (BndrInSingleton (⁻ h ː ¹ν ‗ T1 ⁔ m → T2)).
-              assert (bndr_IsDest (⁻ h ː ¹ν ‗ T1 ⁔ m → T2)). exact (H H0). destruct H1.
+              assert (exists h0 m0 T n, ᶜ{ ⁻ h ː ¹ν ‗ T1 ⁔ m → T2} = ᶜ{ ⁺ h0 ː m0 ⌊ T ⌋ n}). destruct (X H). exists h0, m0, T, n. tauto.
+              destruct H0 as (h0 & m0 & T & n & H0). destruct H0.
             (* Case where u is indeed a lambda value *)
             * rename G into Gv2d, t0 into tb, T0 into T1d, m0 into md, T3 into T2d, TYRt into TYRtb, H2 into Validmd, H0 into Gv2dEqGv2, H into LamxtbEqv2, H1 into T1dEqT1, H3 into mdEqm, H4 into T2dEqT2.
               rewrite (eq_sym LamxtbEqv2) in TYRv2, REDu.
               clear mdEqm. clear Validmd. clear T1dEqT1. clear T2dEqT2. clear Gv2dEqGv2. clear md. clear Gv2d. clear T1d. clear T2d.  clear LamxtbEqv2. clear v2.
               assert (ctx_NoHole (ᶜ{ ᵛ x ː m ‗ T1})). unfold ctx_NoHole. intros n H.
-              assert (ctx_Valid (m ᶜ· Gv1)) as ValidSGv1. exact (StimesPreservesValidity m Gv1 Validm ValidGv1).
-              assert (ctx_Valid (Gv2 ⨄ (m ᶜ· Gv1))) as ValidGv2SGv1. admit. (* TODO: Really not easy *)
+              assert (ctx_IsValid (m ᶜ· Gv1)) as ValidSGv1. exact (StimesPreservesValidity m Gv1 Validm ValidGv1).
+              assert (ctx_IsValid (Gv2 ⨄ (m ᶜ· Gv1))) as ValidGv2SGv1. admit. (* TODO: Really not easy *)
               (* Apply SubLemma on u[x := v1] *)
               assert ((Gv2 ⨄ (m ᶜ· Gv1)) ᵗ⊢ tb ᵗ[ x ≔ v1 ] ː T2). exact (SubLemma Gv2 Gv1 x m T2 T1 tb v1 (Ty_term_T (Gv2 ⨄ ᶜ{ ᵛ x ː m ‗ T1}) tb T2 TYRtb (UnionDOVSingVarIsValid Gv2 x m T1 ValidGv2 (InteractPropagatesDestOnlyRight Ge2 Gv2 DestOnlyGe2v2) Validm) (UnionPreservesNoHole Gv2 (ᶜ{ ᵛ x ː m ‗ T1}) NoHoleGv2 (VarSingletonNoHole x m T1))) (Ty_term_T Gv1 (term_Val v1) T1 TYRv1 ValidGv1 NoHoleGv1) Validm ValidGv2SGv1).
+              admit.
               admit.
     - (* TyR_term_PatU *) admit.
     - (* TyR_term_PatS *) admit.
